\documentclass{article}
\usepackage{ucs} 
\usepackage[utf8x]{inputenc} % Включаем поддержку UTF8  
\usepackage{amsmath,amssymb}
\usepackage{tikz}
\usepackage{setspace}
\usepackage{amsfonts}
\usepackage{geometry}
\usepackage{mathtools} % for \mathclap macro
\usepackage{quoting}
\usepackage[russian]{babel}  % Включаем пакет для поддержки русского языка  
\usepackage[a4paper, left=0.5cm, right=0.5cm, top=0cm, bottom=0cm]{geometry}
\begin{document}
\setlength{\parindent}{0pt}
\begin{Large}
    \textsf{\textbf{МатАн ДЗ №4}}
    
    Шамаев Александр    
\end{Large}
\vspace{1cm}

\textsf{\textbf{(a)}}
\[\lim\limits_{n \to \infty} \frac{3n^2 + 2n - 1}{3 - n - 4n^2} = \lim\limits_{n \to \infty} \frac{3 + \overbrace{\frac{2}{n} - \frac{1}{n^2}}^{\text{б.м.}}}{\underbrace{\frac{3}{n^2} - \frac{1}{n}}_{\text{б.м.}
} - 4} = \boxed{- \frac{3}{4}} \]


\textsf{\textbf{(b)}}
\[
\lim\limits_{n \to \infty} n - \frac{3}{\frac{3}{n} - \frac{3}{n^2} + \frac{1}{n^3}} = 
\lim\limits_{n \to \infty} \frac{3 - \frac{3}{n} + \frac{1}{n^2} - 3}{\frac{3}{n} - \frac{3}{n^2} + \frac{1}{n^3}} = \lim\limits_{n \to \infty} \frac{-3 + \overbrace{\frac{1}{n}}^{\text{б.м.}}}{3 - \underbrace{\frac{3}{n} + \frac{1}{n^2}}_{\text{б.м.}}} = \boxed{-1}
\]

\textsf{\textbf{(c)}}
\begin{center}
    
\[
\lim\limits_{n \to \infty} \frac{2n - \sqrt{4n^2 - 1}}{\sqrt{n^2 + 3} - n} = 
\lim\limits_{n \to \infty} \frac{(4n^2 - 4n^2 + 1)(\sqrt{n^2 + 3} + n)}{(\sqrt{n^2 + 3} - n)(\sqrt{n^2 + 3} + n)(2n + \sqrt{4n^2 - 1})} = 
\]
\[
\lim\limits_{n \to \infty} \frac{\sqrt{n^2 + 3} + n}{(n^2 + 3 - n^2)(2n + \sqrt{4n^2 - 1})} = 
\lim\limits_{n \to \infty} \frac{\sqrt{1 + \overbrace{\frac{3}{n^2}}^{\text{б.м.}}} + 1}{3(2 + \sqrt{4 - \underbrace{\frac{1}{n^2}}}_{\text{б.м.}})} = 
 \frac{2}{12} = \boxed{\frac{1}{6}}
\]
\end{center}

\textsf{\textbf{(d)}}
\begin{center}
   \[
   \lim\limits_{n \to \infty} \sqrt[3]{n+1} - \sqrt[3]{n - 1} = 
   \lim\limits_{n \to \infty} \frac{}{} \sqrt[3]{n+1} - \sqrt[3]{n - 1} = 
   \lim\limits_{n \to \infty} \sqrt{n}(\sqrt[3]{1+\underbrace{\frac{1}{n}}_{\text{б.м.}}} - \sqrt[3]{1 - \underbrace{\frac{1}{n}}_{\text{б.м.}})} = \lim\limits_{n \to \infty} \sqrt{n} (1 - 1) = \boxed{0}
   \] 
\end{center}

\textsf{\textbf{(e)}}
\begin{center}
\[
\lim\limits_{n \to \infty} \frac{10^n + n!}{2^n + (n + 1)!} = 
\lim\limits_{n \to \infty} \frac{\frac{10^n}{(n + 1)!} + \frac{n!}{n!(n + 1)}}{\frac{2^n}{(n + 1)!} + 1} = \frac{\text{lim б.м. + lim б.м.}}{1 + \text{lim б.м.}} = \boxed{0}
\]    
\end{center}

\textsf{\textbf{(f)}}
\begin{center}
\[
\lim\limits_{n \to \infty} \frac{\sqrt[n]{8} - 1}{\sqrt[n]{16} - 1} = \lim\limits_{n \to \infty} \frac{2^{\frac{3}{n}} - 1}{2^{\frac{4}{n}} - 1} = \lim\limits_{n \to \infty} \frac{(2^{\frac{1}{n}} - 1)(2^{\frac{2}{n}} + 2^{\frac{1}{n}} + 1)}{(2^{\frac{2}{n}} - 1)(2^{\frac{2}{n}} + 1)} = \lim\limits_{n \to \infty} \frac{(2^{\frac{1}{n}} - 1)(2^{\frac{2}{n}} + 2^{\frac{1}{n}} + 1)}{(2^{\frac{1}{n}} + 1)(2^{\frac{1}{n}} - 1)(2^{\frac{2}{n}} + 1)} = 
\]    
\[
= \lim\limits_{n \to \infty} \frac{2^{\frac{2}{n}} + 2^{\frac{1}{n}} + 1}{2^{\frac{3}{n}} + 2^{\frac{1}{n}} + 2^{\frac{2}{n}} + 1} =^{(\text{арифм. пред.})}
\frac{1 + 1 + 1}{1 + 1 + 1 + 1} = \boxed{\frac{3}{4}}
\]

\end{center}
\end{document}